

Matérn52 Kernel With Derivatives

April 2024

1 Matérn 52 Kernel

$$k(r) = \left(1 + \sqrt{5}r + \frac{5}{3}r^2\right) \exp(-\sqrt{5}r) \quad (1)$$

$$r(\mathbf{x}^m, \mathbf{x}^n) = \sqrt{\sum_d \frac{(x_d^m - x_d^n)^2}{l_d^2}} \quad (2)$$

2 First Derivatives

$$\begin{aligned} \frac{dk}{dr} &= \frac{d\left(1 + \sqrt{5}r + \frac{5}{3}r^2\right)}{dr} \exp(-\sqrt{5}r) + \left(1 + \sqrt{5}r + \frac{5}{3}r^2\right) \frac{d\exp(-\sqrt{5}r)}{dr} = \\ &= \left(\sqrt{5} + \frac{10}{3}r\right) \exp(-\sqrt{5}r) + (-\sqrt{5}) \left(1 + \sqrt{5}r + \frac{5}{3}r^2\right) \exp(-\sqrt{5}r) = \\ &= \left(\sqrt{5} + \frac{10}{3}r\right) \exp(-\sqrt{5}r) - \left(\sqrt{5} + 5r + \frac{5\sqrt{5}}{3}r^2\right) \exp(-\sqrt{5}r) = \\ &= \exp(-\sqrt{5}r) \left(\sqrt{5} + \frac{10}{3}r - \sqrt{5} - 5r - \frac{5\sqrt{5}}{3}r^2\right) = \\ &= \exp(-\sqrt{5}r) \left(-\frac{5}{3}r - \frac{5\sqrt{5}}{3}r^2\right) = \\ &= -\frac{5}{3}r \left(1 + \sqrt{5}r\right) \exp(-\sqrt{5}r) \quad (3) \end{aligned}$$

$$\begin{aligned}
\frac{\partial r}{\partial x_i^n} &= \frac{\partial \left(\sum_d \frac{(x_d^m - x_d^n)^2}{l_d^2} \right)^{\frac{1}{2}}}{\partial x_i^n} = \\
&= \frac{1}{2} \left(\sum_d \frac{(x_d^m - x_d^n)^2}{l_d^2} \right)^{-\frac{1}{2}} \frac{2}{l_i^2} (x_i^m - x_i^n) (-1) = \\
&= -\frac{x_i^m - x_i^n}{r l_i^2} \quad (4)
\end{aligned}$$

$$\begin{aligned}
\frac{\partial r}{\partial x_j^m} &= \frac{\partial \left(\sum_d \frac{(x_d^m - x_d^n)^2}{l_d^2} \right)^{\frac{1}{2}}}{\partial x_j^m} = \\
&= \frac{1}{2} \left(\sum_d \frac{(x_d^m - x_d^n)^2}{l_d^2} \right)^{-\frac{1}{2}} \frac{2}{l_j^2} (x_j^m - x_j^n) = \\
&= \frac{x_j^m - x_j^n}{r l_j^2} \quad (5)
\end{aligned}$$

$$\begin{aligned}
\frac{\partial k}{\partial x_i^n} &= \frac{dk}{dr} \frac{\partial r}{\partial x_i^n} = \\
&= -\frac{5}{3} r (1 + \sqrt{5}r) \exp(-\sqrt{5}r) \left(-\frac{x_i^m - x_i^n}{r l_i^2} \right) = \\
&= \frac{5}{3} (1 + \sqrt{5}r) \exp(-\sqrt{5}r) \left(\frac{x_i^m - x_i^n}{l_i^2} \right) \quad (6)
\end{aligned}$$

3 Second Derivatives

$$\begin{aligned}
\frac{d^2k}{dr^2} &= \frac{d\left(-\frac{5}{3}r(1+\sqrt{5}r)\exp(-\sqrt{5}r)\right)}{dr} = \\
&= \frac{d\left(-\frac{5}{3}r\right)}{dr} (1+\sqrt{5}r)\exp(-\sqrt{5}r) + \\
&\quad \left(-\frac{5}{3}r\right) \frac{d(1+\sqrt{5}r)}{dr} \exp(-\sqrt{5}r) + \left(-\frac{5}{3}r\right) (1+\sqrt{5}r) \frac{d\exp(-\sqrt{5}r)}{dr} = \\
&= -\frac{5}{3}(1+\sqrt{5}r)\exp(-\sqrt{5}r) + \left(-\frac{5}{3}r\right)(\sqrt{5})\exp(-\sqrt{5}r) + \left(-\frac{5}{3}r\right)(1+\sqrt{5}r)(-\sqrt{5})\exp(-\sqrt{5}r) = \\
&= \left(-\frac{5}{3} - \frac{5\sqrt{5}}{3}r\right)\exp(-\sqrt{5}r) - \frac{5\sqrt{5}}{3}r\exp(-\sqrt{5}r) + \left(\frac{5\sqrt{5}}{3}r + \frac{25}{3}r^2\right)\exp(-\sqrt{5}r) = \\
&= \exp(-\sqrt{5}r) \left(-\frac{5}{3} - \frac{5\sqrt{5}}{3}r - \frac{5\sqrt{5}}{3}r + \frac{5\sqrt{5}}{3}r + \frac{25}{3}r^2\right) = \\
&= \exp(-\sqrt{5}r) \left(-\frac{5}{3} - \frac{5\sqrt{5}}{3}r + \frac{25}{3}r^2\right) = \\
&= \frac{5}{3}(5r^2 - \sqrt{5}r - 1)\exp(-\sqrt{5}r) \quad (7)
\end{aligned}$$

$$\begin{aligned}
\frac{\partial}{\partial x_j^m} \frac{\partial r}{\partial x_i^n} &= \frac{\partial}{\partial x_j^m} \left(-\frac{x_i^m - x_i^n}{l_i^2} \left(\frac{1}{r}\right)\right) = \\
&= \frac{\partial}{\partial x_j^m} \left(-\frac{x_i^m - x_i^n}{l_i^2}\right) \frac{1}{r} + \left(-\frac{x_i^m - x_i^n}{l_i^2}\right) \frac{\partial}{\partial x_j^m} \left(\sum_d \frac{(x_d^m - x_d^n)^2}{l_d^2}\right)^{-\frac{1}{2}} = \\
&= -\frac{1}{rl_i^2} \delta_{ij} + \left(-\frac{x_i^m - x_i^n}{l_i^2}\right) \left(-\frac{1}{2}\right) \left(\sum_d \frac{(x_d^m - x_d^n)^2}{l_d^2}\right)^{-\frac{3}{2}} \frac{2}{l_j^2} (x_j^m - x_j^n) = \\
&= \frac{x_j^m - x_j^n}{l_j^2} \frac{x_i^m - x_i^n}{l_i^2} \frac{1}{r^3} - \frac{1}{rl_i^2} \delta_{ij} \quad (8)
\end{aligned}$$

$$\begin{aligned}
\frac{\partial^2 k}{\partial x_j^m \partial x_i^n} &= \frac{\partial}{\partial x_j^m} \left(\frac{\partial k}{\partial x_i^n}\right) = \frac{\partial}{\partial x_j^m} \left(\frac{dk}{dr} \frac{\partial r}{\partial x_i^n}\right) = \\
&\quad \frac{\partial}{\partial x_j^m} \left(\frac{dk}{dr}\right) \frac{\partial r}{\partial x_i^n} + \frac{dk}{dr} \frac{\partial}{\partial x_j^m} \left(\frac{\partial r}{\partial x_i^n}\right) = \\
&= \frac{d}{dr} \left(\frac{dk}{dr}\right) \frac{\partial r}{\partial x_j^m} \frac{\partial r}{\partial x_i^n} + \frac{dk}{dr} \frac{\partial}{\partial x_j^m} \left(\frac{\partial r}{\partial x_i^n}\right) \quad (9)
\end{aligned}$$

Substituting in terms in Equation 9 gives

$$\begin{aligned}
\frac{\partial^2 k}{\partial x_j^m \partial x_i^n} &= \\
&= \frac{5}{3} (5r^2 - \sqrt{5}r - 1) \exp(-\sqrt{5}r) \left(-\frac{x_i^m - x_i^n}{rl_i^2} \right) \left(\frac{x_j^m - x_j^n}{rl_j^2} \right) \\
&\quad + -\frac{5}{3}r (1 + \sqrt{5}r) \exp(-\sqrt{5}r) \left(\frac{x_j^m - x_j^n}{l_j^2} \frac{x_i^m - x_i^n}{l_i^2} \frac{1}{r^3} - \frac{1}{rl_i^2} \delta_{ij} \right) \quad (10)
\end{aligned}$$

To simplify, define b

$$b = \left(\frac{x_i^m - x_i^n}{l_i^2} \right) \left(\frac{x_j^m - x_j^n}{l_j^2} \right) \quad (11)$$

Equation 10 becomes

$$\begin{aligned}
&-\frac{5}{3r^2} (5r^2 - \sqrt{5}r - 1) \exp(-\sqrt{5}r) b - \frac{5}{3}r (1 + \sqrt{5}r) \exp(-\sqrt{5}r) \left(\frac{b}{r^3} - \frac{\delta_{ij}}{rl_i^2} \right) = \\
&= -\frac{5}{3} \exp(-\sqrt{5}r) \left[\frac{b}{r^2} (5r^2 - \sqrt{5}r - 1) + r (1 + \sqrt{5}r) \left(\frac{b}{r^3} - \frac{\delta_{ij}}{rl_i^2} \right) \right] = \\
&= -\frac{5}{3} \exp(-\sqrt{5}r) \left[\frac{5br^2}{r^2} - \frac{\sqrt{5}br}{r^2} - \frac{b}{r^2} + (r + \sqrt{5}r^2) \left(\frac{b}{r^3} - \frac{\delta_{ij}}{rl_i^2} \right) \right] = \\
&= -\frac{5}{3} \exp(-\sqrt{5}r) \left[\frac{5br^2}{r^2} - \frac{\sqrt{5}br}{r^2} - \frac{b}{r^2} + \frac{br}{r^3} - \frac{r\delta_{ij}}{rl_i^2} + \frac{\sqrt{5}br^2}{r^3} - \frac{\sqrt{5}r^2\delta_{ij}}{rl_i^2} \right] = \\
&= -\frac{5}{3} \exp(-\sqrt{5}r) \left[5b - \frac{\sqrt{5}b}{r} - \frac{b}{r^2} + \frac{b}{r^2} - \frac{\delta_{ij}}{l_i^2} + \frac{\sqrt{5}b}{r} - \frac{\sqrt{5}r\delta_{ij}}{l_i^2} \right] = \\
&= -\frac{5}{3} \exp(-\sqrt{5}r) \left[5b - \frac{\delta_{ij}}{l_i^2} - \frac{\sqrt{5}r\delta_{ij}}{l_i^2} \right] = \\
&= -\frac{5}{3} \exp(-\sqrt{5}r) \left[5b - \frac{\delta_{ij}}{l_i^2} (1 + \sqrt{5}r) \right] = \\
&= -\frac{5}{3} \exp(-\sqrt{5}r) \left[5 \left(\frac{x_i^m - x_i^n}{l_i^2} \right) \left(\frac{x_j^m - x_j^n}{l_j^2} \right) - \frac{\delta_{ij}}{l_i^2} (1 + \sqrt{5}r) \right] \quad (12)
\end{aligned}$$

4 Diagonal

For t training points with d input dimensions, the first t entries of the diagonal will be $\text{cov}(f^t, f^t)$. The next td entries will be $\text{cov}(\omega_d^t, \omega_d^t)$. The first t entries will be $k(0) = 1$. When $m = n$ and $i = j$, then $r = 0$, so Equation 12 simplifies to

$$\frac{\partial^2 k}{\partial x_j^m \partial x_j^m} = \frac{5}{3l_j^2} \quad (13)$$